lib/all.fst
@@ -1,0 +1,24 @@
+module All
+open Heap
+open ST
+
+kind AllPre = AllPre_h heap
+kind AllPost (a:Type) = AllPost_h heap a
+kind AllWP (a:Type) = AllWP_h heap a
+new_effect ALL = ALL_h heap
+effect All (a:Type) (pre:AllPre) (post: (heap -> AllPost a)) =
+       ALL a
+           (fun (p:AllPost a) (h:heap) -> pre h /\ (forall ra h1. post h ra h1 ==> p ra h1)) (* AllWP *)
+           (fun (p:AllPost a) (h:heap) -> forall ra h1. (pre h /\ post h ra h1) ==> p ra h1) (* WLP *)
+default effect ML (a:Type) =
+  ALL a (all_null_wp heap a) (all_null_wp heap a)
+sub_effect
+  STATE ~> ALL = fun (a:Type) (wp:STWP a)   (p:AllPost a) -> wp (fun a -> p (V a))
+sub_effect
+  EXN   ~> ALL = fun (a:Type) (wp:ExWP a)   (p:AllPost a) (h:heap) -> wp (fun ra -> p ra h)
+
+assume val pipe_right: 'a -> ('a -> 'b) -> 'b
+assume val pipe_left: ('a -> 'b) -> 'a -> 'b
+assume val failwith: string -> All 'a (fun h -> True) (fun h a h' -> is_Err a /\ h==h')
+assume val exit: int -> 'a
+assume val try_with: (unit -> 'a) -> (exn -> 'a) -> 'a
